main/SolEnv.v
@@ -1,6 +1,0 @@
-Require Import main.Syntax.
-
-Definition ContractsEnv := address -> ContractState.
-Definition Empty_ContractsEnv : ContractsEnv := fun x => Default_ContractState.
-
-Definition c_env := Empty_ContractsEnv.
